Clean/Ironwood.lean
@@ -37,6 +37,7 @@ import Clean.Ironwood.Action.SpendAuthority
 import Clean.Ironwood.Action.AddressIntegrity
 import Clean.Ironwood.Ecc.Chip
 import Clean.Ironwood.Action.Circuit
+import Clean.Ironwood.Action.Bundle
 
 /-!
 # Ironwood circuits
